Completed Facade QueryStructure Examples.

src/Examples/QueryStructure/StocksFacade.v
@@ -6,6 +6,12 @@ Instance : Query_eq (Word.word n) :=
   { A_eq_dec := @Word.weq n }.
 Opaque Word.weq.
 Opaque Word.natToWord.
+Opaque Word.wlt_dec.
+Definition WordMax (w w' : W) :=
+  if Word.wlt_dec w w' then w' else w.
+Definition MaxW (rows : Comp (list W)) : Comp (option W) :=
+  FoldAggregateOption WordMax rows.
+Definition SumW rows := FoldAggregate (@Word.wplus 32) (Word.natToWord 32 0) rows.
 
 Definition Market := W.
 Definition StockType := W.
@@ -29,31 +35,20 @@ Definition TRANSACTIONS := "TRANSACTIONS".
 Definition StocksSchema :=
   Query Structure Schema
     [ relation STOCKS has
-              schema <STOCK_CODE :: StockCode,
-                      FULL_NAME :: string,
-                      MARKET :: Market,
-                      TYPE :: StockType>
+              schema <STOCK_CODE :: W,
+                      FULL_NAME :: W,
+                      MARKET :: W,
+                      TYPE :: W>
               where (UniqueAttribute ``STOCK_CODE); (* uniqueness, really *)
       relation TRANSACTIONS has
               schema <STOCK_CODE :: W,
-                      DATE :: Date,
-                      TIME :: Timestamp,
-                      PRICE :: N,
-                      VOLUME :: N> ]
+                      DATE :: W,
+                      TIME :: W,
+                      PRICE :: W,
+                      VOLUME :: W> ]
     enforcing [attribute STOCK_CODE for TRANSACTIONS references STOCKS].
 
-Definition StocksSig : ADTSig :=
-  ADTsignature {
-      Constructor "Init"               : rep,
-      Method "AddStock"           : rep * (StocksSchema#STOCKS)       -> rep * bool,
-      Method "AddTransaction"     : rep * (StocksSchema#TRANSACTIONS) -> rep * bool,
-      Method "TotalVolume"        : rep * StockCode * Date          -> rep * N,
-      Method "MaxPrice"           : rep * StockCode * Date          -> rep * (option N),
-      Method "TotalActivity"      : rep * StockCode * Date          -> rep * nat,
-      Method "LargestTransaction" : rep * StockType * Date          -> rep * (option N)
-    }.
-
-Definition StocksSpec : ADT StocksSig :=
+Definition StocksSpec : ADT _ :=
   QueryADTRep StocksSchema {
     Def Constructor0 "Init" : rep := empty,
 
@@ -63,51 +58,161 @@ Definition StocksSpec : ADT StocksSig :=
     Def Method1 "AddTransaction" (r : rep) (transaction : StocksSchema#TRANSACTIONS) : rep * bool :=
         Insert transaction into r!TRANSACTIONS,
 
-    Def Method2 "TotalVolume" (r : rep) (code : StockCode) (date : Date) : rep * N :=
-          sum <- SumN (For (transaction in r!TRANSACTIONS)
+    Def Method2 "TotalVolume" (r : rep) (code : StockCode) (date : Date) : rep * W :=
+          sum <- SumW (For (transaction in r!TRANSACTIONS)
                            Where (transaction!STOCK_CODE = code)
                            Where (transaction!DATE = date)
                            Return transaction!VOLUME);
     ret (r, sum),
 
-    Def Method2 "MaxPrice" (r : rep) (code : StockCode) (date : Date) : rep * option N :=
-      max <- MaxN (For (transaction in r!TRANSACTIONS)
+    Def Method2 "MaxPrice" (r : rep) (code : StockCode) (date : Date) : rep * option W :=
+      max <- MaxW (For (transaction in r!TRANSACTIONS)
                        Where (transaction!STOCK_CODE = code)
                        Where (transaction!DATE = date)
                        Return transaction!PRICE);
      ret (r, max),
 
-    Def Method2 "TotalActivity" (r : rep) (code : StockCode) (date : Date) : rep * nat :=
+    Def Method2 "TotalActivity" (r : rep) (code : StockCode) (date : Date) : rep * W :=
        count <- Count (For (transaction in r!TRANSACTIONS)
                            Where (transaction!STOCK_CODE = code)
                            Where (transaction!DATE = date)
                            Return ());
-     ret (r, count),
+     ret (r, Word.natToWord 32 count),
 
-    Def Method2 "LargestTransaction" (r : rep) (type : StockType) (date : Date) : rep * option N :=
-        max <- MaxN (For (stock in r!STOCKS) (transaction in r!TRANSACTIONS)
+    Def Method2 "LargestTransaction" (r : rep) (type : StockType) (date : Date) : rep * option W :=
+        max <- MaxW (For (stock in r!STOCKS) (transaction in r!TRANSACTIONS)
                          Where (stock!TYPE = type)
                          Where (transaction!DATE = date)
                          Where (stock!STOCK_CODE = transaction!STOCK_CODE)
-                         Return (N.mul transaction!PRICE transaction!VOLUME));
+                         Return (Word.wmult transaction!PRICE transaction!VOLUME));
      ret (r, max)
 }%methDefParsing.
 
-
 Definition SharpenedStocks :
-  FullySharpened StocksSpec.
+  MostlySharpened StocksSpec.
 Proof.
-
-  master_plan EqIndexTactics.
-
-  (* Uncomment this to see the mostly sharpened implementation *)
-  (* partial_master_plan EqIndexTactics. *)
-  (*master_plan EqIndexTactics. *)
+  start sharpening ADT.
+  simpl; pose_string_hyps; pose_heading_hyps.
+  start_honing_QueryStructure'.
+  hone method "AddStock".
+  { setoid_rewrite UniqueAttribute_symmetry.
+    setoid_rewrite (@refine_uniqueness_check_into_query' StocksSchema Fin.F1 _ _ _ _).
+    setoid_rewrite refine_Count.
+    simplify with monad laws; simpl in *; subst.
+    setoid_rewrite refine_pick_eq'.
+    setoid_rewrite refine_bind_unit.
+    setoid_rewrite refine_If_Then_Else_Duplicate.
+    finish honing. }
+  GenerateIndexesForAll EqExpressionAttributeCounter
+  ltac:(fun attrlist =>
+          let attrlist' := eval compute in (PickIndexes _ (CountAttributes' attrlist)) in
+              make_simple_indexes attrlist'
+                                  ltac:(LastCombineCase6 BuildEarlyEqualityIndex)
+                                         ltac:(LastCombineCase5 BuildLastEqualityIndex)).
+  + plan EqIndexUse createEarlyEqualityTerm createLastEqualityTerm
+         EqIndexUse_dep createEarlyEqualityTerm_dep createLastEqualityTerm_dep.
+  + setoid_rewrite refine_For_rev; simplify with monad laws.
+    plan EqIndexUse createEarlyEqualityTerm createLastEqualityTerm
+         EqIndexUse_dep createEarlyEqualityTerm_dep createLastEqualityTerm_dep.
+  + setoid_rewrite refine_For_rev; simplify with monad laws.
+    plan EqIndexUse createEarlyEqualityTerm createLastEqualityTerm
+         EqIndexUse_dep createEarlyEqualityTerm_dep createLastEqualityTerm_dep.
+  + setoid_rewrite refine_For_rev; simplify with monad laws.
+    plan EqIndexUse createEarlyEqualityTerm createLastEqualityTerm
+         EqIndexUse_dep createEarlyEqualityTerm_dep createLastEqualityTerm_dep.
+  + setoid_rewrite refine_For_rev; simplify with monad laws.
+    plan EqIndexUse createEarlyEqualityTerm createLastEqualityTerm
+         EqIndexUse_dep createEarlyEqualityTerm_dep createLastEqualityTerm_dep.
+  + setoid_rewrite refine_For_rev; simplify with monad laws.
+    plan EqIndexUse createEarlyEqualityTerm createLastEqualityTerm
+         EqIndexUse_dep createEarlyEqualityTerm_dep createLastEqualityTerm_dep.
+  + setoid_rewrite refine_For_rev; simplify with monad laws.
+    plan EqIndexUse createEarlyEqualityTerm createLastEqualityTerm
+         EqIndexUse_dep createEarlyEqualityTerm_dep createLastEqualityTerm_dep.
+  + hone method "AddStock".
+    { simpl in *; subst.
+      simplify with monad laws.
+      unfold ilist2_hd at 1; simpl.
+      repeat setoid_rewrite rev_length.
+      repeat setoid_rewrite map_length.
+      setoid_rewrite refine_pick_eq'; simplify with monad laws.
+      repeat setoid_rewrite refine_If_Then_Else_Bind.
+      repeat setoid_rewrite refineEquiv_bind_bind.
+      repeat setoid_rewrite refineEquiv_bind_unit; simpl.
+      unfold H1; eapply refine_under_bind; intros; set_evars.
+      rewrite (CallBagFind_fst H0); simpl.
+      finish honing.
+    }
+    hone method "AddTransaction".
+    { simpl in *; subst.
+      setoid_rewrite refine_Count; simplify with monad laws.
+      setoid_rewrite app_nil_r;
+        setoid_rewrite map_map; simpl.
+      unfold ilist2_hd at 1; simpl.
+      setoid_rewrite rev_length.
+      setoid_rewrite map_length.
+      setoid_rewrite refine_pick_eq'; simplify with monad laws.
+      repeat setoid_rewrite refine_If_Then_Else_Bind.
+      repeat setoid_rewrite refineEquiv_bind_bind.
+      repeat setoid_rewrite refineEquiv_bind_unit; simpl.
+      unfold H1.
+      eapply refine_under_bind; intros; set_evars.
+      rewrite (CallBagFind_fst H0); simpl.
+      finish honing.
+    }
+    hone method "TotalVolume".
+    { simpl in *; subst; simplify with monad laws.
+      unfold H1; eapply refine_under_bind; intros; set_evars.
+      rewrite (CallBagFind_fst H0); simpl.
+      setoid_rewrite refine_pick_eq'; simplify with monad laws.
+      rewrite app_nil_r, map_map; unfold ilist2_hd; simpl.
+      finish honing.
+    }
+    hone method "MaxPrice".
+    { simpl in *; subst; simplify with monad laws.
+      unfold H1; eapply refine_under_bind; intros; set_evars.
+      rewrite (CallBagFind_fst H0); simpl.
+      setoid_rewrite refine_pick_eq'; simplify with monad laws.
+      rewrite app_nil_r, map_map; unfold ilist2_hd; simpl.
+      finish honing.
+    }
+    hone method "TotalActivity".
+    { simpl in *; subst.
+      setoid_rewrite refine_Count; simplify with monad laws.
+      unfold H1; eapply refine_under_bind; intros; set_evars.
+      rewrite (CallBagFind_fst H0); simpl.
+      setoid_rewrite refine_pick_eq'; simplify with monad laws.
+      rewrite app_nil_r, map_map; unfold ilist2_hd; simpl.
+      rewrite rev_length, map_length.
+      finish honing.
+    }
+    hone method "LargestTransaction".
+    { simpl in *; subst; simplify with monad laws.
+      unfold H1; eapply refine_under_bind; intros; set_evars. 
+      rewrite (CallBagFind_fst H0); simpl.
+      etransitivity.
+      eapply refine_under_bind_both.
+      eapply (@foo StocksSchema Index (Fin.FS Fin.F1)).
+      intros; finish honing.
+      simplify with monad laws.
+      unfold H2; apply refine_under_bind; set_evars.
+      intros.
+      apply foo' in H4; rewrite H4.
+      setoid_rewrite refine_pick_eq'; simplify with monad laws.
+      simpl.
+      finish honing.
+    }
+    simpl; eapply reflexivityT.
+  + unfold CallBagFind, CallBagInsert.
+    pose_headings_all.
+    match goal with
+    | |- appcontext[ @BuildADT (IndexedQueryStructure ?Schema ?Indexes) ] =>
+      FullySharpenQueryStructure Schema Indexes
+    end.
 
 Time Defined.
 (* 2590MB  *)
 
-Time Definition StocksImpl : ComputationalADT.cADT StocksSig :=
-  Eval simpl in projT1 SharpenedStocks.
-(* 3728MB *)
+Time Definition StocksImpl :=
+  Eval simpl in (fst (projT1 SharpenedStocks)).
 Print StocksImpl.
